move expr_rel to a separate file, and demand the substitution to be truly closing

theories/simplang/ctx.v
@@ -2,7 +2,7 @@
 
 From simuliris.simulation Require Import slsls lifting.
 From simuliris.simplang Require Import proofmode tactics.
-From simuliris.simplang Require Import heapbij_refl.
+From simuliris.simplang Require Import heap_bij heapbij_refl.
 
 (** First we need to define a notion of "contexts"
 (more general than the 'evaluation contexts' that the language comes with) *)
@@ -83,3 +83,80 @@ Local Definition fill_item (Ci : ctx_item) (e : expr) : expr :=
 Definition ctx := list ctx_item.
 Definition fill_ctx (C : ctx) (e : expr) : expr :=
   foldl (flip fill_item) e C.
+
+Section ctx.
+  Context `{sbijG Σ}.
+  (* TODO: do the same thing for a general notion of contexts *)
+  Import simp_lang. (* bring simp_lang contexts back into priority. *)
+
+  Definition ectxi_wf (Ki : ectx_item) : Prop :=
+    match Ki with
+    | LetCtx _ e => expr_wf e
+    | UnOpCtx _ => True
+    | BinOpLCtx _ v => val_wf v
+    | BinOpRCtx _ e => expr_wf e
+    | IfCtx e1 e2 => expr_wf e1 ∧ expr_wf e2
+    | PairLCtx v => val_wf v
+    | PairRCtx e => expr_wf e
+    | FstCtx | SndCtx | InjLCtx | InjRCtx | LoadCtx _ => True
+    | MatchCtx _ e1 _ e2 => expr_wf e1 ∧ expr_wf e2
+    | AllocNLCtx v => val_wf v
+    | AllocNRCtx e => expr_wf e
+    | FreeNLCtx v => val_wf v
+    | FreeNRCtx e => expr_wf e
+    | StoreLCtx _ v => val_wf v
+    | StoreRCtx _ e => expr_wf e
+    | CmpXchgLCtx _ _ => False  (* unsupported *)
+    | CmpXchgMCtx _ _ => False  (* unsupported *)
+    | CmpXchgRCtx _ _ => False  (* unsupported *)
+    | FaaLCtx _ => False  (* unsupported *)
+    | FaaRCtx _ => False (* unsupported *)
+    | CallLCtx v => val_wf v
+    | CallRCtx e => expr_wf e
+    end.
+  (* we do not use [Forall] since that does not compute,
+    making applications of [heap_bij_ectx_refl] hard. *)
+  Fixpoint ectx_wf (K : ectx) : Prop :=
+    match K with
+    | [] => True
+    | Ki :: K => ectxi_wf Ki ∧ ectx_wf K
+    end.
+
+  (* FIXME: old proof relied on using [expr_rel] with a non-closing subst map
+  Theorem heap_bij_ectx_refl π K :
+    ectx_wf K → ⊢ sim_ectx val_rel π K K val_rel.
+  Proof.
+    intros Hwf. iInduction (K) as [ | Ki K] "IH".
+    { iIntros (v_t v_s) "Hv". sim_pures. by sim_val. }
+    destruct Hwf as [Hiwf Kwf].
+    iSpecialize ("IH" with "[//]").
+    iIntros (v_t v_s) "#Hv". destruct Ki; sim_pures; iApply sim_bind; (iApply sim_wand; [ iApply expr_rel_empty | iApply "IH"]).
+    - iApply expr_rel_let; [by iApply expr_rel_val | by iApply expr_wf_sound].
+    - iApply expr_rel_call; [by iApply expr_rel_val | iApply expr_wf_sound; apply Hiwf].
+    - iApply expr_rel_call; [iApply expr_wf_sound; apply Hiwf | by iApply expr_rel_val ].
+    - iApply expr_rel_unop. by iApply expr_rel_val.
+    - iApply expr_rel_binop; [by iApply expr_rel_val | by iApply expr_wf_sound].
+    - iApply expr_rel_binop; [ by iApply expr_wf_sound | by iApply expr_rel_val].
+    - iApply expr_rel_if; [by iApply expr_rel_val | iApply expr_wf_sound; apply Hiwf..].
+    - iApply expr_rel_pair; iApply expr_rel_val; [done | by iApply val_wf_sound].
+    - iApply expr_rel_pair; [by iApply expr_wf_sound | by iApply expr_rel_val].
+    - iApply expr_rel_fst; by iApply expr_rel_val.
+    - iApply expr_rel_snd; by iApply expr_rel_val.
+    - iApply expr_rel_injl; by iApply expr_rel_val.
+    - iApply expr_rel_injr; by iApply expr_rel_val.
+    - iApply expr_rel_match; [by iApply expr_rel_val | iApply expr_wf_sound; apply Hiwf..].
+    - iApply expr_rel_allocN; [by iApply expr_rel_val | iApply expr_rel_val; by iApply val_wf_sound].
+    - iApply expr_rel_allocN; [iApply expr_wf_sound; apply Hiwf | by iApply expr_rel_val ].
+    - iApply expr_rel_freeN; [by iApply expr_rel_val | iApply expr_wf_sound; apply Hiwf].
+    - iApply expr_rel_freeN; [iApply expr_wf_sound; apply Hiwf | by iApply expr_rel_val ].
+    - iApply expr_rel_load; by iApply expr_rel_val.
+    - iApply expr_rel_store; [by iApply expr_rel_val | iApply expr_wf_sound; apply Hiwf].
+    - iApply expr_rel_store; [iApply expr_wf_sound; apply Hiwf | by iApply expr_rel_val ].
+    - by destruct Hiwf.
+    - by destruct Hiwf.
+    - by destruct Hiwf.
+    - by destruct Hiwf.
+    - by destruct Hiwf.
+  Qed. *)
+
+End ctx.
